TODO: check various crappy defs (hd nil allowed, ...) and finish patterns

2016/Ext_Structures.thy
@@ -19,24 +19,25 @@ text{* In this section,we extend our current lambda calculus with extended struc
 
 inductive Lmatch ::"Lpattern \<Rightarrow> lterm \<Rightarrow> (lterm \<Rightarrow>lterm) \<Rightarrow> bool" where
   M_Var:
-    "is_value_L v \<Longrightarrow> Lmatch (V n) v (fill (\<lambda>p. if (p=n) then v else (<|V p|>)))" |
+    "is_value_L v \<Longrightarrow> Lmatch (V n as A) v (fill (\<lambda>p. if (p=n) then v else (<|V p as A|>)))" |
   M_RCD:
     "distinct L \<Longrightarrow> length L = length LT \<Longrightarrow> length F = length PL \<Longrightarrow> length PL = length LT 
     \<Longrightarrow> is_value_L (Record L LT) \<Longrightarrow> (\<And>i. i<length PL \<Longrightarrow> Lmatch (PL!i) (LT!i) (F!i))
     \<Longrightarrow> Lmatch (RCD L PL) (Record L LT) (\<Odot> F)"
 
-inductive Lmatch_Gnl ::"Lpattern \<Rightarrow> lterm \<Rightarrow> (lterm \<Rightarrow>lterm) \<Rightarrow> bool" where
+inductive Lmatch_Type ::"Lpattern \<Rightarrow> (nat \<rightharpoonup> ltype) \<Rightarrow> bool" where
   M_Var:
-    "Lmatch_Gnl (V n) v (fill (\<lambda>p. if (p=n) then v else (<|V p|>)))" |
+    "Lmatch_Type (V n as A) [n \<mapsto> A]" |
   M_RCD:
-    "distinct L \<Longrightarrow> length F = length PL \<Longrightarrow> length L = length PL \<Longrightarrow> (\<And>i. i<length PL \<Longrightarrow> Lmatch_Gnl (PL!i) (ProjR (L!i) t) (F!i))
-    \<Longrightarrow> Lmatch_Gnl (RCD L PL) t (\<Odot> F)"
+    "distinct L \<Longrightarrow> length Tx = length PL \<Longrightarrow> length L = length PL \<Longrightarrow> 
+      (\<And>i. i<length PL \<Longrightarrow> Lmatch_Type (PL!i) (Tx!i))
+    \<Longrightarrow> Lmatch_Type (RCD L PL) (\<Odot>\<^sub>T Tx)"
 
 inductive coherent ::"Lpattern \<Rightarrow> ltype \<Rightarrow> bool" where
- "coherent (V n) A" |
- "L\<noteq>[] \<Longrightarrow> length PL = length L \<Longrightarrow> length TL = length L \<Longrightarrow> distinct (Pvars (RCD L PL)) \<Longrightarrow>
-    (\<And>i. i<length PL\<Longrightarrow> coherent (PL!i) (TL!i)) \<Longrightarrow>
-    coherent (RCD L PL) (\<lparr>L|:|TL\<rparr>)"
+ "coherent (V n as A) A" |
+ "distinct(Pvars (RCD L PL)) \<Longrightarrow> length L = length PL \<Longrightarrow> length PL = length TL \<Longrightarrow>
+  (\<And>i. i<length TL \<Longrightarrow> coherent (PL!i) (TL!i)) \<Longrightarrow> coherent (RCD L PL) (\<lparr>L|:|TL\<rparr>)"
+  
 
 inductive eval1_L :: "lterm \<Rightarrow> lterm \<Rightarrow> bool" where
   -- "Rules relating to the evaluation of Booleans"
@@ -55,15 +56,6 @@ inductive eval1_L :: "lterm \<Rightarrow> lterm \<Rightarrow> bool" where
   eval1_LApp_LAbs:
     "is_value_L v2 \<Longrightarrow> eval1_L (LApp (LAbs T' t12) v2)
       (shift_L (-1) 0 (subst_L 0 (shift_L 1 0 v2) t12))" |
-
-  -- "Rules relating to the evaluation of Plus"
-  eval1_LPlus:
-    "eval1_L (LPlus (LNat n1) (LNat n2)) (LNat (n1+n2))"|
-  eval1_LUMinus:
-    "eval1_L (UMinus (LNat n1)) (LNat (-n1))" |
-  eval1_LIsZero:
-    "eval1_L (IsZero (LNat 0)) LTrue" |
- -- "Rules relating to evaluation of sequence"
   
   eval1_L_Seq:
     "eval1_L t1 t1' \<Longrightarrow> eval1_L (Seq t1 t2) (Seq t1' t2)" |
@@ -155,7 +147,7 @@ inductive eval1_L :: "lterm \<Rightarrow> lterm \<Rightarrow> bool" where
     "eval1_L t t1 \<Longrightarrow> eval1_L (Ltail A t) (Ltail A t1)" 
 
 type_synonym lcontext = "ltype list"
-type_synonym pcontext = "(lterm \<Rightarrow> lterm)"
+type_synonym pcontext = "(nat \<rightharpoonup> ltype)"
 
 notation Nil ("\<emptyset>")
 abbreviation cons :: "lcontext \<Rightarrow> ltype \<Rightarrow> lcontext" (infixl "|,|" 200) where
@@ -172,81 +164,87 @@ text{*  For the typing rule of letbinder, we require to replace the type
 inductive has_type_L :: "lcontext \<Rightarrow> lterm \<Rightarrow> pcontext \<Rightarrow> ltype \<Rightarrow> bool" ("((_)/ \<turnstile> \<lparr>(_)|;|(_)\<rparr>/ |:| (_))" [150, 150, 150, 150] 150) where
   -- "Rules relating to the type of Booleans"
   has_type_LTrue:
-    "\<Gamma> \<turnstile> \<lparr>LTrue|;|fill \<sigma>\<rparr> |:| Bool" |
+    "\<Gamma> \<turnstile> \<lparr>LTrue|;| \<sigma>\<rparr> |:| Bool" |
   has_type_LFalse:
-    "\<Gamma> \<turnstile> \<lparr>LFalse|;|fill \<sigma>\<rparr> |:| Bool" |
+    "\<Gamma> \<turnstile> \<lparr>LFalse|;| \<sigma>\<rparr> |:| Bool" |
   has_type_LIf:
-    "\<Gamma> \<turnstile> \<lparr>t1|;|fill \<sigma>\<rparr> |:| Bool \<Longrightarrow> \<Gamma> \<turnstile> \<lparr>t2|;|fill \<sigma>\<rparr> |:| T' \<Longrightarrow> \<Gamma> \<turnstile> \<lparr>t3|;|fill \<sigma>\<rparr> |:| T' \<Longrightarrow> \<Gamma> \<turnstile> \<lparr>LIf t1 t2 t3|;|fill \<sigma>\<rparr> |:| T'" |
+    "\<Gamma> \<turnstile> \<lparr>t1|;| \<sigma>\<rparr> |:| Bool \<Longrightarrow> \<Gamma> \<turnstile> \<lparr>t2|;| \<sigma>\<rparr> |:| T' \<Longrightarrow> \<Gamma> \<turnstile> \<lparr>t3|;| \<sigma>\<rparr> |:| T' \<Longrightarrow> 
+      \<Gamma> \<turnstile> \<lparr>LIf t1 t2 t3|;| \<sigma>\<rparr> |:| T'" |
 
   -- \<open>Rules relating to the type of the constructs of the $\lambda$-calculus\<close>
   has_type_LVar:
-    "(x, T') |\<in>| \<Gamma> \<Longrightarrow> \<Gamma> \<turnstile> \<lparr>LVar x|;|fill \<sigma>\<rparr> |:| (T')" |
-  has_type_LNat:
-    "\<Gamma> \<turnstile> \<lparr>LNat n|;| fill \<sigma>\<rparr> |:| Nat"|
-  has_type_LPlus:
-    "\<Gamma> \<turnstile> \<lparr>t1|;| fill \<sigma>\<rparr> |:| Nat \<Longrightarrow> \<Gamma> \<turnstile> \<lparr>t2|;| fill \<sigma>\<rparr> |:| Nat \<Longrightarrow> \<Gamma> \<turnstile> \<lparr>LPlus t1 t2|;| fill \<sigma>\<rparr> |:| Nat" |  
-  has_type_UMinus:
-    "\<Gamma> \<turnstile> \<lparr>t|;| fill \<sigma>\<rparr> |:| Nat \<Longrightarrow> \<Gamma> \<turnstile> \<lparr>UMinus t|;| fill \<sigma>\<rparr> |:| Nat" |
-  has_type_IsZero:
-    "\<Gamma> \<turnstile> \<lparr>t|;| fill \<sigma>\<rparr> |:| Nat \<Longrightarrow> \<Gamma> \<turnstile> \<lparr>IsZero t|;| fill \<sigma>\<rparr> |:| Bool" |
+    "(x, T') |\<in>| \<Gamma> \<Longrightarrow> \<Gamma> \<turnstile> \<lparr>LVar x|;| \<sigma>\<rparr> |:| (T')" |
   has_type_LAbs:
-    "(\<Gamma> |,| T1) \<turnstile> \<lparr>t2|;| fill \<sigma>\<rparr> |:| T2 \<Longrightarrow> \<Gamma> \<turnstile> \<lparr>LAbs T1 t2|;|fill \<sigma>\<rparr> |:| (T1 \<rightarrow> T2)" |
+    "(\<Gamma> |,| T1) \<turnstile> \<lparr>t2|;| \<sigma>\<rparr> |:| T2 \<Longrightarrow> \<Gamma> \<turnstile> \<lparr>LAbs T1 t2|;| \<sigma>\<rparr> |:| (T1 \<rightarrow> T2)" |
   has_type_LApp:
-    "\<Gamma> \<turnstile> \<lparr>t1|;|fill \<sigma>\<rparr> |:| (T11 \<rightarrow> T12) \<Longrightarrow> \<Gamma> \<turnstile> \<lparr>t2|;|fill \<sigma>\<rparr> |:| T11 \<Longrightarrow> \<Gamma> \<turnstile> \<lparr>LApp t1 t2|;|fill \<sigma>\<rparr> |:| T12" |  
+    "\<Gamma> \<turnstile> \<lparr>t1|;| \<sigma>\<rparr> |:| (T11 \<rightarrow> T12) \<Longrightarrow> \<Gamma> \<turnstile> \<lparr>t2|;| \<sigma>\<rparr> |:| T11 \<Longrightarrow> 
+      \<Gamma> \<turnstile> \<lparr>LApp t1 t2|;| \<sigma>\<rparr> |:| T12" |  
   has_type_LUnit:
-    "\<Gamma> \<turnstile> \<lparr>unit|;|fill \<sigma>\<rparr> |:| Unit " |  
+    "\<Gamma> \<turnstile> \<lparr>unit|;| \<sigma>\<rparr> |:| Unit " |  
   has_type_LSeq:
-    "\<Gamma> \<turnstile> \<lparr>t1|;|fill \<sigma>\<rparr> |:| Unit \<Longrightarrow> \<Gamma> \<turnstile> \<lparr>t2|;|fill \<sigma>\<rparr> |:| A \<Longrightarrow> \<Gamma> \<turnstile> \<lparr>Seq t1 t2|;|fill \<sigma>\<rparr> |:| A" |
+    "\<Gamma> \<turnstile> \<lparr>t1|;| \<sigma>\<rparr> |:| Unit \<Longrightarrow> \<Gamma> \<turnstile> \<lparr>t2|;| \<sigma>\<rparr> |:| A \<Longrightarrow> \<Gamma> \<turnstile> \<lparr>Seq t1 t2|;| \<sigma>\<rparr> |:| A" |
   has_type_LAscribe:
-    "\<Gamma> \<turnstile> \<lparr>t1|;|fill \<sigma>\<rparr> |:| A \<Longrightarrow> \<Gamma> \<turnstile> \<lparr>t1 as A|;|fill \<sigma>\<rparr> |:| A" |
+    "\<Gamma> \<turnstile> \<lparr>t1|;| \<sigma>\<rparr> |:| A \<Longrightarrow> \<Gamma> \<turnstile> \<lparr>t1 as A|;| \<sigma>\<rparr> |:| A" |
   has_type_Let:
-    "\<Gamma> \<turnstile> \<lparr>t1|;|fill \<sigma>\<rparr> |:| A \<Longrightarrow> (insert_nth x A \<Gamma>) \<turnstile> \<lparr> t2|;| fill \<sigma>\<rparr> |:| B \<Longrightarrow> \<Gamma> \<turnstile> \<lparr>Let var x := t1 in t2|;|fill \<sigma>\<rparr> |:| B" |
+    "\<Gamma> \<turnstile> \<lparr>t1|;| \<sigma>\<rparr> |:| A \<Longrightarrow> (insert_nth x A \<Gamma>) \<turnstile> \<lparr> t2|;| \<sigma>\<rparr> |:| B \<Longrightarrow> 
+      \<Gamma> \<turnstile> \<lparr>Let var x := t1 in t2|;| \<sigma>\<rparr> |:| B" |
   has_type_Pair:
-    "\<Gamma> \<turnstile> \<lparr>t1|;|fill \<sigma>\<rparr> |:| A \<Longrightarrow> \<Gamma> \<turnstile> \<lparr>t2|;|fill \<sigma>\<rparr> |:| B \<Longrightarrow> \<Gamma> \<turnstile> \<lparr>\<lbrace>t1,t2\<rbrace>|;|fill \<sigma>\<rparr> |:| A |\<times>| B" |
+    "\<Gamma> \<turnstile> \<lparr>t1|;| \<sigma>\<rparr> |:| A \<Longrightarrow> \<Gamma> \<turnstile> \<lparr>t2|;| \<sigma>\<rparr> |:| B \<Longrightarrow> 
+      \<Gamma> \<turnstile> \<lparr>\<lbrace>t1,t2\<rbrace>|;| \<sigma>\<rparr> |:| A |\<times>| B" |
   has_type_Proj1:
-    "\<Gamma> \<turnstile> \<lparr>t1|;|fill \<sigma>\<rparr> |:| A |\<times>| B \<Longrightarrow> \<Gamma> \<turnstile> \<lparr>\<pi>1 t1|;|fill \<sigma>\<rparr> |:| A" |
+    "\<Gamma> \<turnstile> \<lparr>t1|;| \<sigma>\<rparr> |:| A |\<times>| B \<Longrightarrow> \<Gamma> \<turnstile> \<lparr>\<pi>1 t1|;| \<sigma>\<rparr> |:| A" |
   has_type_Proj2:
-    "\<Gamma> \<turnstile> \<lparr>t1|;|fill \<sigma>\<rparr> |:| A |\<times>| B \<Longrightarrow> \<Gamma> \<turnstile> \<lparr>\<pi>2 t1|;|fill \<sigma>\<rparr> |:| B" |
+    "\<Gamma> \<turnstile> \<lparr>t1|;| \<sigma>\<rparr> |:| A |\<times>| B \<Longrightarrow> \<Gamma> \<turnstile> \<lparr>\<pi>2 t1|;| \<sigma>\<rparr> |:| B" |
   has_type_Tuple:
-    "L\<noteq>[] \<Longrightarrow> length L = length TL \<Longrightarrow> (\<And>i. 0\<le>i \<Longrightarrow> i< length L \<Longrightarrow> \<Gamma> \<turnstile> \<lparr>(L ! i)|;|fill \<sigma>\<rparr> |:| (TL ! i))
-      \<Longrightarrow> \<Gamma> \<turnstile> \<lparr>Tuple L|;|fill \<sigma>\<rparr> |:| \<lparr>TL\<rparr>" |
+    "L\<noteq>[] \<Longrightarrow> length L = length TL \<Longrightarrow> 
+      (\<And>i. 0\<le>i \<Longrightarrow> i< length L \<Longrightarrow> \<Gamma> \<turnstile> \<lparr>(L ! i)|;| \<sigma>\<rparr> |:| (TL ! i))
+      \<Longrightarrow> \<Gamma> \<turnstile> \<lparr>Tuple L|;| \<sigma>\<rparr> |:| \<lparr>TL\<rparr>" |
   has_type_ProjT:
-    "1\<le>i \<Longrightarrow> i\<le> length TL \<Longrightarrow> \<Gamma> \<turnstile> \<lparr>t|;|fill \<sigma>\<rparr> |:| \<lparr>TL\<rparr> \<Longrightarrow> \<Gamma> \<turnstile> \<lparr>\<Pi> i t|;|fill \<sigma>\<rparr> |:| (TL ! (i-1))" |
+    "1\<le>i \<Longrightarrow> i\<le> length TL \<Longrightarrow> \<Gamma> \<turnstile> \<lparr>t|;| \<sigma>\<rparr> |:| \<lparr>TL\<rparr> \<Longrightarrow> 
+      \<Gamma> \<turnstile> \<lparr>\<Pi> i t|;| \<sigma>\<rparr> |:| (TL ! (i-1))" |
   has_type_RCD:
-    "L\<noteq>[] \<Longrightarrow> distinct L \<Longrightarrow> length LT = length TL \<Longrightarrow> length L = length LT \<Longrightarrow> (\<And>i. i< length LT \<Longrightarrow> \<Gamma> \<turnstile> \<lparr>(LT ! i)|;|fill \<sigma>\<rparr> |:| (TL ! i))
-      \<Longrightarrow> \<Gamma> \<turnstile> \<lparr>Record L LT|;|fill \<sigma>\<rparr> |:| \<lparr>L|:|TL\<rparr>" |
+    "L\<noteq>[] \<Longrightarrow> distinct L \<Longrightarrow> length LT = length TL \<Longrightarrow> length L = length LT \<Longrightarrow>
+      (\<And>i. i< length LT \<Longrightarrow> \<Gamma> \<turnstile> \<lparr>(LT ! i)|;| \<sigma>\<rparr> |:| (TL ! i))
+      \<Longrightarrow> \<Gamma> \<turnstile> \<lparr>Record L LT|;| \<sigma>\<rparr> |:| \<lparr>L|:|TL\<rparr>" |
   has_type_ProjR:
-    "distinct L1 \<Longrightarrow> l\<in> set L1  \<Longrightarrow> length L1 = length TL \<Longrightarrow> \<Gamma> \<turnstile> \<lparr>t|;|fill \<sigma>\<rparr> |:| \<lparr>L1|:|TL\<rparr> \<Longrightarrow> \<Gamma> \<turnstile> \<lparr>ProjR l t|;|fill \<sigma>\<rparr> |:| (TL ! index L1 l)" |
+    "distinct L1 \<Longrightarrow> l\<in> set L1  \<Longrightarrow> length L1 = length TL \<Longrightarrow> 
+      \<Gamma> \<turnstile> \<lparr>t|;| \<sigma>\<rparr> |:| \<lparr>L1|:|TL\<rparr> \<Longrightarrow> 
+      \<Gamma> \<turnstile> \<lparr>ProjR l t|;| \<sigma>\<rparr> |:| (TL ! index L1 l)" |
   has_type_PatternVar:
-    "\<Gamma> \<turnstile> \<lparr> \<sigma> k |;| fill \<sigma> \<rparr> |:| A \<Longrightarrow> \<Gamma> \<turnstile> \<lparr><|V k|>|;|fill \<sigma>\<rparr> |:| A" |
+    "\<sigma> k = Some A \<Longrightarrow> \<Gamma> \<turnstile> \<lparr><|V k as A|>|;| \<sigma>\<rparr> |:| A" |
   has_type_LetPattern:
-    "coherent p B \<Longrightarrow> Lmatch_Gnl p t1 \<sigma> \<Longrightarrow> \<Gamma> \<turnstile> \<lparr>t1|;| fill \<sigma>1\<rparr> |:| B \<Longrightarrow>
-     \<Gamma> \<turnstile> \<lparr>t2|;|((fill \<sigma>1) \<circ> \<sigma>)\<rparr> |:| A \<Longrightarrow> \<Gamma> \<turnstile> \<lparr>Let pattern p := t1 in t2|;|fill \<sigma>1\<rparr> |:| A" |
+    "coherent p B\<Longrightarrow> Lmatch_Type p \<sigma> \<Longrightarrow> \<Gamma> \<turnstile> \<lparr>t1|;| \<sigma>1\<rparr> |:| B \<Longrightarrow>
+     \<Gamma> \<turnstile> \<lparr>t2|;|(\<sigma> ++ \<sigma>1)\<rparr> |:| A \<Longrightarrow> \<Gamma> \<turnstile> \<lparr>Let pattern p := t1 in t2|;| \<sigma>1\<rparr> |:| A" |
   has_type_Inl:
-    "\<Gamma> \<turnstile> \<lparr>t1|;|fill \<sigma>1\<rparr> |:| A \<Longrightarrow> \<Gamma> \<turnstile> \<lparr>inl t1 as A|+|B |;|fill \<sigma>1\<rparr> |:| A|+|B" |
+    "\<Gamma> \<turnstile> \<lparr>t1|;| \<sigma>1\<rparr> |:| A \<Longrightarrow> \<Gamma> \<turnstile> \<lparr>inl t1 as A|+|B |;|\<sigma>1\<rparr> |:| A|+|B" |
   has_type_Inr:
-    "\<Gamma> \<turnstile> \<lparr>t1|;|fill \<sigma>1\<rparr> |:| B \<Longrightarrow> \<Gamma> \<turnstile> \<lparr>inr t1 as A|+|B |;|fill \<sigma>1\<rparr> |:| A|+|B" |
+    "\<Gamma> \<turnstile> \<lparr>t1|;| \<sigma>1\<rparr> |:| B \<Longrightarrow> \<Gamma> \<turnstile> \<lparr>inr t1 as A|+|B |;| \<sigma>1\<rparr> |:| A|+|B" |
   has_type_Case:
-    "\<Gamma> \<turnstile> \<lparr> t|;|fill \<sigma>1 \<rparr> |:| A|+|B \<Longrightarrow> insert_nth x A \<Gamma> \<turnstile> \<lparr>t1|;|fill \<sigma>1\<rparr> |:| C \<Longrightarrow>
-     insert_nth y B \<Gamma> \<turnstile> \<lparr>t2|;|fill \<sigma>1\<rparr> |:| C \<Longrightarrow> \<Gamma> \<turnstile> \<lparr>Case t of Inl x \<Rightarrow> t1 | Inr y \<Rightarrow> t2 |;|fill \<sigma>1\<rparr> |:| C" |
+    "\<Gamma> \<turnstile> \<lparr> t|;| \<sigma>1 \<rparr> |:| A|+|B \<Longrightarrow> insert_nth x A \<Gamma> \<turnstile> \<lparr>t1|;| \<sigma>1\<rparr> |:| C \<Longrightarrow>
+     insert_nth y B \<Gamma> \<turnstile> \<lparr>t2|;| \<sigma>1\<rparr> |:| C \<Longrightarrow> 
+     \<Gamma> \<turnstile> \<lparr>Case t of Inl x \<Rightarrow> t1 | Inr y \<Rightarrow> t2 |;| \<sigma>1\<rparr> |:| C" |
   has_type_Variant:
-    "\<Gamma> \<turnstile> \<lparr> t |;| fill \<sigma> \<rparr> |:| (TL!i) \<Longrightarrow> \<Gamma> \<turnstile> \<lparr> <(L!i):=t> as <L|,|TL> |;| fill \<sigma> \<rparr> |:| <L|,|TL>" |
+    "\<Gamma> \<turnstile> \<lparr> t |;| \<sigma> \<rparr> |:| (TL!i) \<Longrightarrow> 
+      \<Gamma> \<turnstile> \<lparr> <(L!i):=t> as <L|,|TL> |;|\<sigma> \<rparr> |:| <L|,|TL>" |
   has_type_CaseV:
-    " L\<noteq>\<emptyset> \<Longrightarrow> length I = length L \<Longrightarrow> length L = length TL \<Longrightarrow> length L = length LT \<Longrightarrow>
-      \<Gamma> \<turnstile> \<lparr> t |;| fill \<sigma> \<rparr> |:| <L|,|TL> \<Longrightarrow> (\<forall>i<length L. insert_nth (I!i) (TL!i) \<Gamma> \<turnstile> \<lparr>(LT!i)|;|fill \<sigma>\<rparr> |:| A) \<Longrightarrow>
-      \<Gamma> \<turnstile> \<lparr> Case t of <L:=I> \<Rightarrow> LT |;|fill \<sigma>\<rparr> |:| A" |
+    " L\<noteq>\<emptyset> \<Longrightarrow> length I = length L \<Longrightarrow> length L = length TL \<Longrightarrow> 
+      length L = length LT \<Longrightarrow>
+      \<Gamma> \<turnstile> \<lparr> t |;| \<sigma> \<rparr> |:| <L|,|TL> \<Longrightarrow> 
+      (\<forall>i<length L. insert_nth (I!i) (TL!i) \<Gamma> \<turnstile> \<lparr>(LT!i)|;| \<sigma>\<rparr> |:| A) \<Longrightarrow>
+      \<Gamma> \<turnstile> \<lparr> Case t of <L:=I> \<Rightarrow> LT |;| \<sigma>\<rparr> |:| A" |
   has_type_Fix:
-    "\<Gamma> \<turnstile> \<lparr> t |;| fill \<sigma> \<rparr> |:| A\<rightarrow>A \<Longrightarrow> \<Gamma> \<turnstile> \<lparr> fix t |;| fill \<sigma> \<rparr> |:| A"|
+    "\<Gamma> \<turnstile> \<lparr> t |;| \<sigma>\<rparr> |:| A\<rightarrow>A \<Longrightarrow> \<Gamma> \<turnstile> \<lparr> fix t |;| \<sigma>\<rparr> |:| A"|
   has_type_Nil:
-    "\<Gamma> \<turnstile> \<lparr> Lnil A |;| fill \<sigma> \<rparr> |:| \<lambda>List A"|
+    "\<Gamma> \<turnstile> \<lparr> Lnil A |;| \<sigma>\<rparr> |:| \<lambda>List A"|
   has_type_isNil:
-    "\<Gamma> \<turnstile> \<lparr> t|;| fill \<sigma> \<rparr> |:| \<lambda>List A \<Longrightarrow>\<Gamma> \<turnstile> \<lparr> Lisnil A t|;| fill \<sigma> \<rparr> |:| Bool"| 
+    "\<Gamma> \<turnstile> \<lparr> t|;| \<sigma> \<rparr> |:| \<lambda>List A \<Longrightarrow>\<Gamma> \<turnstile> \<lparr> Lisnil A t|;| \<sigma> \<rparr> |:| Bool"| 
   has_type_head:
-    "\<Gamma> \<turnstile> \<lparr> t|;| fill \<sigma> \<rparr> |:| \<lambda>List A \<Longrightarrow>\<Gamma> \<turnstile> \<lparr> Lhead A t|;| fill \<sigma> \<rparr> |:| A"| 
+    "\<Gamma> \<turnstile> \<lparr> t|;| \<sigma> \<rparr> |:| \<lambda>List A \<Longrightarrow>\<Gamma> \<turnstile> \<lparr> Lhead A t|;| \<sigma> \<rparr> |:| A"| 
   has_type_tail:
-    "\<Gamma> \<turnstile> \<lparr> t|;| fill \<sigma> \<rparr> |:| \<lambda>List A \<Longrightarrow>\<Gamma> \<turnstile> \<lparr> Ltail A t|;| fill \<sigma> \<rparr> |:| A"| 
+    "\<Gamma> \<turnstile> \<lparr> t|;| \<sigma> \<rparr> |:| \<lambda>List A \<Longrightarrow>\<Gamma> \<turnstile> \<lparr> Ltail A t|;| \<sigma> \<rparr> |:| A"| 
   has_type_cons:
-    "\<Gamma> \<turnstile> \<lparr> t|;| fill \<sigma> \<rparr> |:| A \<Longrightarrow> \<Gamma> \<turnstile> \<lparr> t' |;| fill \<sigma> \<rparr> |:| A \<Longrightarrow>\<Gamma> \<turnstile> \<lparr> Lcons A t t'|;| fill \<sigma> \<rparr> |:| \<lambda>List A"  
+    "\<Gamma> \<turnstile> \<lparr> t|;| \<sigma> \<rparr> |:| A \<Longrightarrow> \<Gamma> \<turnstile> \<lparr> t' |;| \<sigma> \<rparr> |:| A \<Longrightarrow>
+      \<Gamma> \<turnstile> \<lparr> Lcons A t t'|;| \<sigma> \<rparr> |:| \<lambda>List A"  
 
 inductive_cases has_type_LetE : "\<Gamma> \<turnstile> \<lparr> Let var x := t1 in t2|;|\<sigma>1\<rparr>  |:| B"
 inductive_cases has_type_ProjTE: "\<Gamma> \<turnstile> \<lparr> \<Pi> i t|;|\<sigma>1\<rparr> |:| R"
@@ -254,7 +252,7 @@ inductive_cases has_type_ProjRE: "\<Gamma> \<turnstile> \<lparr> ProjR l t|;|\<s
 inductive_cases has_type_LetPE: "\<Gamma> \<turnstile> \<lparr>Let pattern p := t1 in t2|;|\<sigma>1\<rparr> |:| A"
 inductive_cases has_type_CaseSE: "\<Gamma> \<turnstile> \<lparr>Case t of Inl x \<Rightarrow> t1 | Inr y \<Rightarrow> t2|;|\<sigma>1\<rparr> |:| R"
 inductive_cases has_type_CaseVE: "\<Gamma> \<turnstile> \<lparr>Case t of <L:=I> \<Rightarrow> LT|;|\<sigma>1\<rparr> |:| R"
-inductive_cases has_type_LAbsE: "\<Gamma> \<turnstile> \<lparr>LAbs T1 t2|;|fill \<sigma>'\<rparr> |:| R"
+inductive_cases has_type_LAbsE: "\<Gamma> \<turnstile> \<lparr>LAbs T1 t2|;|\<sigma>1\<rparr> |:| R"
 inductive_cases has_type_VariantE: "\<Gamma> \<turnstile> \<lparr><l:=t> as R |;|\<sigma>1\<rparr> |:| R"
 
 lemma record_patterns_characterisation:
@@ -266,7 +264,7 @@ lemma inversion:
   "\<Gamma> \<turnstile> \<lparr> LFalse |;| \<sigma>\<rparr> |:| R \<Longrightarrow> R = Bool"
   "\<Gamma> \<turnstile> \<lparr> LIf t1 t2 t3 |;| \<sigma>\<rparr> |:| R \<Longrightarrow>  \<Gamma> \<turnstile> \<lparr>t1|;| \<sigma>\<rparr> |:| Bool \<and> \<Gamma> \<turnstile> \<lparr>t2|;| \<sigma>\<rparr> |:| R \<and> \<Gamma> \<turnstile> \<lparr>t3|;| \<sigma>\<rparr> |:| R"
   "\<Gamma> \<turnstile> \<lparr> LVar x|;| \<sigma>\<rparr> |:| R \<Longrightarrow> (x, R) |\<in>| \<Gamma>"
-  "\<Gamma> \<turnstile> \<lparr> LAbs T1 t2 |;| fill \<sigma>'\<rparr> |:| R \<Longrightarrow> \<exists>R2. R = T1 \<rightarrow> R2 \<and>  \<Gamma> |,| T1 \<turnstile> \<lparr>t2|;|fill \<sigma>'\<rparr> |:| R2 "
+  "\<Gamma> \<turnstile> \<lparr> LAbs T1 t2 |;| \<sigma>\<rparr> |:| R \<Longrightarrow> \<exists>R2. R = T1 \<rightarrow> R2 \<and>  \<Gamma> |,| T1 \<turnstile> \<lparr>t2|;| \<sigma>\<rparr> |:| R2 "
   "\<Gamma> \<turnstile> \<lparr> LApp t1 t2 |;| \<sigma>\<rparr> |:| R \<Longrightarrow> \<exists>T11. \<Gamma> \<turnstile> \<lparr>t1|;| \<sigma>\<rparr> |:| T11 \<rightarrow> R \<and> \<Gamma> \<turnstile> \<lparr>t2|;| \<sigma>\<rparr> |:| T11"
   "\<Gamma> \<turnstile> \<lparr> unit|;| \<sigma>\<rparr> |:| R \<Longrightarrow> R = Unit"
   "\<Gamma> \<turnstile> \<lparr> Seq t1 t2 |;| \<sigma>\<rparr> |:| R \<Longrightarrow> \<exists>A. R = A \<and> \<Gamma> \<turnstile> \<lparr>t2|;| \<sigma>\<rparr> |:| A \<and> \<Gamma> \<turnstile> \<lparr>t1|;| \<sigma>\<rparr> |:| Unit"
@@ -281,9 +279,9 @@ lemma inversion:
                                     (\<forall>i. 0\<le>i \<longrightarrow> i< length LT \<longrightarrow> \<Gamma> \<turnstile> \<lparr> (LT ! i)|;| \<sigma>\<rparr> |:| (TL ! i)) " 
   "\<Gamma> \<turnstile> \<lparr> (ProjR l t)|;| \<sigma>\<rparr> |:| R \<Longrightarrow>\<exists>m L TL. \<Gamma> \<turnstile> \<lparr>t |;| \<sigma>\<rparr> |:| \<lparr>L|:|TL\<rparr> \<and> index L l = m \<and> TL ! m = R \<and> distinct L \<and> length L = length TL
                               \<and> l \<in> set L"
-  "\<Gamma> \<turnstile> \<lparr><|V k|>|;|\<sigma>\<rparr> |:| R \<Longrightarrow> \<Gamma> \<turnstile> \<lparr>\<sigma> (<|V k|>)|;| \<sigma>\<rparr> |:| R"
-  "\<Gamma> \<turnstile> \<lparr>Let pattern p := t1 in t2|;|\<sigma>1\<rparr> |:| R \<Longrightarrow>\<exists>\<sigma> B. coherent p B\<and> Lmatch_Gnl p t1 \<sigma>  \<and> \<Gamma> \<turnstile> \<lparr>t1|;|\<sigma>1\<rparr> |:| B \<and>
-                                                  \<Gamma> \<turnstile> \<lparr>t2|;|(\<sigma>1 \<circ> \<sigma>)\<rparr> |:| R" 
+  "\<Gamma> \<turnstile> \<lparr><|V k as A|>|;|\<sigma>\<rparr> |:| R \<Longrightarrow> \<sigma> k = Some A"
+  "\<Gamma> \<turnstile> \<lparr>Let pattern p := t1 in t2|;|\<sigma>1\<rparr> |:| R \<Longrightarrow>\<exists>\<sigma> B. coherent p B\<and> Lmatch_Type p \<sigma>  \<and> \<Gamma> \<turnstile> \<lparr>t1|;|\<sigma>1\<rparr> |:| B \<and>
+                                                  \<Gamma> \<turnstile> \<lparr>t2|;|(\<sigma> ++  \<sigma>1)\<rparr> |:| R" 
   "\<Gamma> \<turnstile> \<lparr>inl t as R|;|\<sigma>1\<rparr> |:| R \<Longrightarrow>\<exists>A B. R = A|+|B \<and> \<Gamma> \<turnstile> \<lparr>t|;|\<sigma>1\<rparr> |:| A"
   "\<Gamma> \<turnstile> \<lparr>inr t as R|;|\<sigma>1\<rparr> |:| R \<Longrightarrow>\<exists>A B. R = A|+|B \<and> \<Gamma> \<turnstile> \<lparr>t|;|\<sigma>1\<rparr> |:| B"
   "\<Gamma> \<turnstile> \<lparr>Case t of Inl x \<Rightarrow> t1 | Inr y \<Rightarrow> t2|;|\<sigma>1\<rparr> |:| R \<Longrightarrow>\<exists>A B C. R = C \<and> \<Gamma> \<turnstile> \<lparr>t|;|\<sigma>1\<rparr> |:| A|+|B \<and>
@@ -298,7 +296,7 @@ proof -
     by fastforce 
 next
   assume H1: "\<Gamma> \<turnstile> \<lparr>Let pattern p := t1 in t2|;|\<sigma>1\<rparr> |:| R"
-  show "\<exists>\<sigma> B. coherent p B\<and> Lmatch_Gnl p t1 \<sigma>  \<and> \<Gamma> \<turnstile> \<lparr>t1|;|\<sigma>1\<rparr> |:| B \<and> \<Gamma> \<turnstile> \<lparr>t2|;|(\<sigma>1 \<circ> \<sigma>)\<rparr> |:| R"
+  show "\<exists>\<sigma> B. coherent p B \<and> Lmatch_Type p \<sigma>  \<and> \<Gamma> \<turnstile> \<lparr>t1|;|\<sigma>1\<rparr> |:| B \<and> \<Gamma> \<turnstile> \<lparr>t2|;|(\<sigma> ++ \<sigma>1)\<rparr> |:| R"
     using has_type_LetPE[OF H1]
     by metis
 next
@@ -313,16 +311,7 @@ next
     by metis    
 next
   assume H5: "\<Gamma> \<turnstile> \<lparr>Case t of <L1:=I> \<Rightarrow> LT|;|\<sigma>1\<rparr> |:| A"
-  have "\<And>TL \<sigma>. \<sigma>1 = fill \<sigma> \<Longrightarrow> length L1 = length TL \<Longrightarrow>\<forall>i<length TL. (take (I ! i) \<Gamma> @ \<emptyset> |,| (TL ! i) @ drop (I ! i) \<Gamma>) \<turnstile> \<lparr>(LT ! i)|;|fill \<sigma>\<rparr> |:| A
-         \<Longrightarrow> \<forall>i<length L1. insert_nth (I ! i) (TL ! i) \<Gamma> \<turnstile> \<lparr>(LT ! i)|;|\<sigma>1\<rparr> |:| A"
-    proof (rule+)
-      fix TL \<sigma> i
-      assume hyps:"\<forall>i<length TL. (take (I ! i) \<Gamma> @ \<emptyset> |,| (TL ! i) @ drop (I ! i) \<Gamma>) \<turnstile> \<lparr>(LT ! i)|;|fill \<sigma>\<rparr> |:| A"
-                  "\<sigma>1 = fill \<sigma>" "i<length L1" "length L1 = length TL"
-      then show "insert_nth (I ! i) (TL ! i) \<Gamma> \<turnstile> \<lparr>(LT ! i)|;|\<sigma>1\<rparr> |:| A"
-        by fastforce  
-    qed      
-  then show "\<exists>TL. L1\<noteq>\<emptyset> \<and> length I = length L1 \<and> length L1 = length TL \<and> length L1 = length LT \<and>
+  show "\<exists>TL. L1\<noteq>\<emptyset> \<and> length I = length L1 \<and> length L1 = length TL \<and> length L1 = length LT \<and>
       \<Gamma> \<turnstile> \<lparr> t |;| \<sigma>1 \<rparr> |:| <L1|,|TL> \<and> (\<forall>i<length L1. insert_nth (I!i) (TL!i) \<Gamma> \<turnstile> \<lparr>(LT!i)|;| \<sigma>1\<rparr> |:| A)"
     using has_type_CaseVE[OF H5]
     by (metis append_Cons append_Nil insert_nth_take_drop)
@@ -334,40 +323,6 @@ lemma[simp]: "nat (1 + int x) = Suc x" by simp
 
 lemma[simp]: "nat (int x - 1) = x - 1" by simp 
 
-lemma shift_fill:
-  "fill \<sigma> (shift_L d c t) = shift_L d c (fill \<sigma> t)"
-sorry
-
-lemma unfold_SV_sub:
-  "length d = length c \<Longrightarrow> 
-   rec_nat id (\<lambda>n r. r \<circ> shift_L ((d @ [d1]) ! n) ((c @ [c1]) ! n)) (length d) t =
-   unfold_SV d c t"
-sorry
-
-lemma fill_unfold:
-  "length d = length c \<Longrightarrow>fill \<sigma> (unfold_SV d c t) = unfold_SV d c (fill \<sigma> t)"
-proof (induction "length d" arbitrary: c d t)
-  case (Suc n)
-    obtain d1 c1 d' c' where unfolds:"d=d'@[d1]" "c=c'@[c1]"
-      using Suc(2,3) 
-      by (metis append_butlast_last_id length_0_conv nat.simps(3))
-    hence sub_len:"length d' = length c'" "n=length d'" using Suc(2,3) by auto
-    
-    from Suc(3) have lhs1:"fill \<sigma> (unfold_SV d c t) = fill \<sigma> (rec_nat id (\<lambda>n r. r \<circ> shift_L ((d' @ [d1]) ! n) ((c' @ [c1]) ! n)) (length c')
-       (shift_L ((d' @ [d1]) ! length c') c1 t))"
-      by (simp add: unfolds)
-    from Suc(3) have "unfold_SV d c (fill \<sigma> t) = 
-        rec_nat id (\<lambda>n r. r \<circ> shift_L ((d' @ [d1]) ! n) ((c' @ [c1]) ! n)) (length c')
-         (shift_L ((d' @ [d1]) ! length c') c1 (fill \<sigma> t))"
-      by (simp add: unfolds)
-    with lhs1 show ?case
-      using Suc(1)[OF sub_len(2,1), of "shift_L d1 c1 t"
-                    , unfolded sub_len(1)[symmetric] shift_fill , simplified]
-            unfold_SV_sub[OF sub_len(1), of d1 c1, 
-                          unfolded unfolds[symmetric] Suc(3) sub_len(1), simplified, 
-                          unfolded unfolds sub_len(1)[symmetric]] 
-      by (simp add: sub_len(1)[symmetric]) 
-qed auto
 
 lemma fill_fill_comp:
   "fill \<sigma> \<circ> fill \<sigma>1 = fill (fill \<sigma> \<circ> \<sigma>1)"
@@ -377,210 +332,131 @@ proof (rule)
     proof (induction x arbitrary: \<sigma> \<sigma>1)
       case (Pattern p)
         show ?case
-          proof (induction p)
-            case (SV d c k)
-              show ?case
-                using fill_unfold[of d c \<sigma> "\<sigma>1 k"]
-                by auto
-          qed auto
-    qed auto
+          by (induction p, simp+)
+    qed simp+
 qed
 
-lemma lmatchGnl_gives_fill:
-  "Lmatch_Gnl p t \<sigma> \<Longrightarrow> coherent p A \<Longrightarrow> \<exists>\<sigma>1. fill \<sigma>1 = \<sigma>" 
-proof (induction arbitrary: A rule: Lmatch_Gnl.induct)
-  case (M_RCD L F PL t)
-    show ?case
-      using M_RCD(2,3,5,6)
-      proof (induction F arbitrary:PL L A)
-        case Nil
-          thus ?case by (auto simp: coherent.simps[of "RCD \<emptyset> _", simplified])
-      next
-        case (Cons f F)
-          obtain p PL' where unfold_PL:"PL = p#PL'"
-            using Cons(2) length_Suc_conv
-            by metis
-          then obtain l L' where unfold_L: "L= l#L'"
-            using Cons(3) length_Suc_conv
-            by metis
-          obtain TL where H:"A = \<lparr>(l # L')|:|TL\<rparr>"
-                          "length (p # PL') = length (l # L')"
-                          "length TL = length (l # L')"
-                          "distinct (list_iter op @ \<emptyset> (map Pvars (p # PL')))"
-                          "\<And>x. x<length (p # PL') \<Longrightarrow> coherent ((p # PL') ! x) (TL ! x)"
-            using Cons(5)[unfolded unfold_L unfold_PL coherent.simps[of "RCD _ _", simplified]]
-            by auto
-          obtain \<Sigma> where BigCirc_\<Sigma>:"L'\<noteq>[] \<Longrightarrow>fill \<Sigma> = \<Odot> F"
-            using Cons(1)[OF  Cons(2)[unfolded unfold_PL, simplified]
-                              Cons(3)[unfolded unfold_L unfold_PL, simplified],
-                          of "\<lparr>L'|:| (drop 1 TL)\<rparr>"
-                          ]                   
-                  Cons(4)[of "_+1", unfolded unfold_PL unfold_L, simplified]
-                  "coherent.intros"(2)[of L' PL' "drop 1 TL"]      
-                  length_drop[of 1 TL] H(2,3,4)[simplified] nth_drop[of 1 _ TL, symmetric, simplified]
-                  H(5)[of "_+1", simplified]
-             by fastforce
-          obtain \<sigma>1 where "fill \<sigma>1 = f"
-            using Cons(4)[of 0 "_!0"] Cons(2) 
-                  Cons(5)[unfolded coherent.simps[of "RCD _ _", simplified]]
-            by force
-          with BigCirc_\<Sigma> show ?case
-            using fill_fill_comp[of \<sigma>1 \<Sigma>]
-                  Cons(2,3)[unfolded unfold_L]
-            by (cases "L'=[]")
-               (metis BigCirc.simps(1) BigCirc.simps(2) comp_id length_0_conv length_Cons nat.simps(1),
-                 auto)
-      qed
-qed auto
-
-
-
-(*lemma weakening1 :
-  fixes \<Gamma>::lcontext  and t::lterm and A R::ltype and \<sigma> \<sigma>'::"nat\<Rightarrow>lterm"
-  assumes well_typed: "\<Gamma> \<turnstile> \<lparr>t|;|fill \<sigma>\<rparr> |:| A" and
-          shifted_filling:"p\<in>set (patterns t) \<Longrightarrow> \<Gamma> \<turnstile> \<lparr><|V p|>|;|fill \<sigma>\<rparr> |:| R \<Longrightarrow> \<Gamma> \<turnstile> \<lparr><|V p|>|;|fill \<sigma>'\<rparr> |:| R"
-  shows "\<Gamma> \<turnstile> \<lparr>t |;| fill \<sigma>'\<rparr> |:| A"
-sorry*)
-
-
-
-lemma P_list_conv_nth:"(\<And>x. x\<in> A\<union>set L \<Longrightarrow> P x) \<Longrightarrow> (\<And>i. i<length L \<Longrightarrow> P (L!i))"
-using set_conv_nth by auto
-
 lemma weakening :
-  fixes \<Gamma>::lcontext  and t::lterm and A S::ltype and \<sigma> ::"nat\<Rightarrow>lterm" and n::nat
-  assumes well_typed: "\<Gamma> \<turnstile> \<lparr>t|;|fill \<sigma>\<rparr> |:| A" and
+  fixes \<Gamma>::lcontext  and t::lterm and A S::ltype and \<sigma> ::"nat\<rightharpoonup>ltype" and n::nat
+  assumes well_typed: "\<Gamma> \<turnstile> \<lparr>t|;| \<sigma>\<rparr> |:| A" and
           weaker_ctx: " n \<le> length \<Gamma>" 
-  shows "insert_nth n S \<Gamma> \<turnstile> \<lparr>shift_L 1 n t|;|fill \<sigma>\<rparr> |:| A"
+  shows "insert_nth n S \<Gamma> \<turnstile> \<lparr>shift_L 1 n t|;| \<sigma>\<rparr> |:| A"
 using assms 
-proof(induction \<Gamma> t "fill \<sigma>" A arbitrary: n \<sigma> rule:has_type_L.induct)
+proof(induction \<Gamma> t \<sigma> A arbitrary: n rule:has_type_L.induct)
   case (has_type_LAbs \<Gamma>1 T1 t2 \<sigma>1 T2)
     
-    have "Suc n\<le>length(\<Gamma>1|,|T1)" using has_type_LAbs(4) by auto
+    have "Suc n\<le>length(\<Gamma>1|,|T1)" using has_type_LAbs(3) by auto
 
-    hence "insert_nth (Suc n) S (\<Gamma>1 |,| T1) \<turnstile> \<lparr>shift_L 1 (Suc n) t2|;|fill \<sigma>\<rparr> |:| T2"
-      using has_type_LAbs(2)[OF has_type_LAbs(3)] 
-      by fast
+    hence "insert_nth (Suc n) S (\<Gamma>1 |,| T1) \<turnstile> \<lparr>shift_L 1 (Suc n) t2|;| \<sigma>1\<rparr> |:| T2"
+      using has_type_LAbs(2)[where n="Suc n"]
+      by auto
     then show ?case
-      using "has_type_L.intros"(9)[of T1 "insert_nth n S \<Gamma>1" "shift_L 1 n t2" \<sigma> T2]
-            has_type_L.has_type_LAbs 
-      by auto              
+      by (auto intro: has_type_L.has_type_LAbs)              
 next 
   case(has_type_Tuple L TL \<Gamma>1 \<sigma>1)
     show ?case    
       using has_type_Tuple(1,2) nth_map[of _ L "shift_L 1 n"] 
-            has_type_Tuple(4)[OF _ _ has_type_Tuple(5,6)]
-      by (force intro!: has_type_L.intros(18))+
+            has_type_Tuple(4)[OF _ _ has_type_Tuple(5)]
+      by (force intro!: has_type_L.intros(14))+
 next
   case (has_type_ProjT i TL \<Gamma>1 t \<sigma>1)
     show ?case
-      using has_type_ProjT(4)[OF has_type_ProjT(5,6)]
-            "has_type_L.intros"(19)[OF has_type_ProjT(1,2)]
+      using has_type_ProjT(4)[OF has_type_ProjT(5)]
+            "has_type_L.intros"(15)[OF has_type_ProjT(1,2)]
       by fastforce
 next
   case (has_type_RCD L LT TL \<Gamma> \<sigma>1)
     show ?case
       using has_type_RCD(1-4) nth_map[of _ LT "shift_L 1 n"]
-            has_type_RCD(6)[OF _ has_type_RCD(7,8)]           
-      by (force intro!: "has_type_L.intros"(20))+
+            has_type_RCD(6)[OF _ has_type_RCD(7)]           
+      by (force intro!: "has_type_L.intros"(16))+
 next
   case (has_type_Let \<Gamma> t1 \<sigma>1 A x t2 B)
     
-    have "n \<le> x \<Longrightarrow> (take n \<Gamma> @ drop n \<Gamma> |,| S) \<turnstile> \<lparr>Let var Suc x := shift_L 1 n t1 in shift_L 1 n t2|;|fill \<sigma>\<rparr> |:| B"
-      using has_type_Let(2)[OF has_type_Let(5,6)] has_type_Let(6)
-            has_type_Let(4)[unfolded length_insert_nth, OF has_type_Let(5), of n] 
-            insert_nth_comp(1)[OF has_type_Let(6), of x S A] 
-      by (auto intro!: has_type_L.intros(14))  
+    have "n \<le> x \<Longrightarrow> (take n \<Gamma> @ drop n \<Gamma> |,| S) \<turnstile> \<lparr>Let var Suc x := shift_L 1 n t1 in shift_L 1 n t2|;| \<sigma>1\<rparr> |:| B"
+      using has_type_Let(5) has_type_Let(3)
+            has_type_Let(4)[unfolded length_insert_nth,  of n] 
+            insert_nth_comp(1)[OF has_type_Let(5), of x S A] 
+      by (auto intro!: has_type_L.intros(10))  
     then show ?case
-      using has_type_Let(2)[OF has_type_Let(5,6)] 
-            has_type_Let(4)[unfolded length_insert_nth, OF has_type_Let(5), of "Suc n" ] 
-            has_type_Let(6)
-            insert_nth_comp(2)[OF has_type_Let(6),of x S A]  
-      by (auto intro!: has_type_L.intros(14)) 
+      using has_type_Let(3)[OF has_type_Let(5)] 
+            has_type_Let(4)[unfolded length_insert_nth, of "Suc n" ] 
+            has_type_Let(5)
+            insert_nth_comp(2)[OF has_type_Let(5),of x S A]  
+      by (auto intro!: has_type_L.intros(10)) 
 next
-  case (has_type_LetPattern p B t1 \<sigma>1 \<Gamma> \<sigma>2 t2 A \<sigma>3 n)
+  case (has_type_LetPattern p B t1 \<sigma>1 \<Gamma> \<sigma>2 t2 A)
     note hyps=this
-    obtain \<sigma>' where fill_\<sigma>1:"\<sigma>1 = fill \<sigma>'"
-      using lmatchGnl_gives_fill[OF has_type_LetPattern(2,1)]
-      by auto
-      
     show ?case
-      using fill_\<sigma>1
-      apply auto
-      apply rule
-      using hyps(1)
-      apply force
-      defer
-      using hyps(4)[OF hyps(7,8), unfolded shift_fill[symmetric] hyps(7)]
-      apply force
-      using hyps(6)[OF _ hyps(8), of "fill \<sigma>2 \<circ> \<sigma>'", unfolded hyps(7) fill_fill_comp[symmetric]]
-      apply force    
-      
-      (*by (auto intro: has_type_L.intros(24))*) sorry
+      using hyps(1,2) hyps(5)[OF hyps(7)]
+            hyps(6)[OF hyps(7)]
+      by (auto intro: has_type_L.intros(19))
 next
   case (has_type_Case \<Gamma>1 t \<sigma>1 A B x t1 C y t2)
 
 
-    have Sum_type: "insert_nth n S \<Gamma>1 \<turnstile> \<lparr>shift_L 1 n t|;|fill \<sigma>\<rparr> |:| A |+| B"
-      using has_type_Case(2)[OF has_type_Case(7,8)] 
+    have Sum_type: "insert_nth n S \<Gamma>1 \<turnstile> \<lparr>shift_L 1 n t|;| \<sigma>1\<rparr> |:| A |+| B"
+      using has_type_Case(4)[OF has_type_Case(7)] 
       by auto
 
-    have B1:"n \<le> x \<Longrightarrow> n \<le> y \<Longrightarrow> insert_nth (Suc x) A (insert_nth n S \<Gamma>1) \<turnstile> \<lparr>shift_L 1 n t1|;|fill \<sigma>\<rparr> |:| C \<and>
-                                  insert_nth (Suc y) B (insert_nth n S \<Gamma>1) \<turnstile> \<lparr>shift_L 1 n t2|;|fill \<sigma>\<rparr> |:| C"
-      using  has_type_Case(4)[OF has_type_Case(7),of n ] has_type_Case(8)
-             has_type_Case(6)[OF has_type_Case(7),of n ]
+    have B1:"n \<le> x \<Longrightarrow> n \<le> y \<Longrightarrow> insert_nth (Suc x) A (insert_nth n S \<Gamma>1) \<turnstile> \<lparr>shift_L 1 n t1|;|\<sigma>1\<rparr> |:| C \<and>
+                                  insert_nth (Suc y) B (insert_nth n S \<Gamma>1) \<turnstile> \<lparr>shift_L 1 n t2|;|\<sigma>1\<rparr> |:| C"
+      using  has_type_Case(5)[of n] has_type_Case(7)
+             has_type_Case(6)[of n]
              insert_nth_comp(1)[of n \<Gamma>1 _ S _] length_insert_nth
       by (metis le_SucI)+
 
-    have B2: " n \<le> x \<Longrightarrow> \<not> n \<le> y \<Longrightarrow> insert_nth (Suc x) A (insert_nth n S \<Gamma>1) \<turnstile> \<lparr>shift_L 1 n t1|;|fill \<sigma>\<rparr> |:| C \<and> 
-                                      insert_nth y B (insert_nth n S \<Gamma>1) \<turnstile> \<lparr>shift_L 1 (Suc n) t2|;|fill \<sigma>\<rparr> |:| C"
-      using  has_type_Case(4)[OF has_type_Case(7),of n, unfolded length_insert_nth]
-             has_type_Case(6)[OF has_type_Case(7),of "Suc n", unfolded length_insert_nth]  
-             has_type_Case(8) insert_nth_comp[of n \<Gamma>1 _ S _] 
+    have B2: " n \<le> x \<Longrightarrow> \<not> n \<le> y \<Longrightarrow> insert_nth (Suc x) A (insert_nth n S \<Gamma>1) \<turnstile> \<lparr>shift_L 1 n t1|;|\<sigma>1\<rparr> |:| C \<and> 
+                                      insert_nth y B (insert_nth n S \<Gamma>1) \<turnstile> \<lparr>shift_L 1 (Suc n) t2|;|\<sigma>1\<rparr> |:| C"
+      using  has_type_Case(5)[of n, unfolded length_insert_nth]
+             has_type_Case(6)[of "Suc n", unfolded length_insert_nth]  
+             has_type_Case(7) insert_nth_comp[of n \<Gamma>1 _ S _] 
       by (metis Suc_le_mono not_le le_SucI)+
 
-    have B3: "\<not> n \<le> x \<Longrightarrow>  n \<le> y \<Longrightarrow> insert_nth x A (insert_nth n S \<Gamma>1) \<turnstile> \<lparr>shift_L 1 (Suc n) t1|;|fill \<sigma>\<rparr> |:| C \<and>
-                                      insert_nth (Suc y) B (insert_nth n S \<Gamma>1) \<turnstile> \<lparr>shift_L 1 n t2|;|fill \<sigma>\<rparr> |:| C"
-      using  has_type_Case(4)[OF has_type_Case(7) ,of "Suc n", unfolded length_insert_nth]
-             has_type_Case(6)[OF has_type_Case(7) ,of n, unfolded length_insert_nth]  
-             has_type_Case(8) insert_nth_comp[of n \<Gamma>1 _ S _] 
+    have B3: "\<not> n \<le> x \<Longrightarrow>  n \<le> y \<Longrightarrow> insert_nth x A (insert_nth n S \<Gamma>1) \<turnstile> \<lparr>shift_L 1 (Suc n) t1|;|\<sigma>1\<rparr> |:| C \<and>
+                                      insert_nth (Suc y) B (insert_nth n S \<Gamma>1) \<turnstile> \<lparr>shift_L 1 n t2|;|\<sigma>1\<rparr> |:| C"
+      using  has_type_Case(5)[of "Suc n", unfolded length_insert_nth]
+             has_type_Case(6)[of n, unfolded length_insert_nth]  
+             has_type_Case(7) insert_nth_comp[of n \<Gamma>1 _ S _] 
       by (metis Suc_le_mono not_le le_SucI)+
 
-    have B4: "\<not> n \<le> x \<Longrightarrow> \<not> n \<le> y \<Longrightarrow> insert_nth x A (insert_nth n S \<Gamma>1) \<turnstile> \<lparr>shift_L 1 (Suc n) t1|;|fill \<sigma>\<rparr> |:| C \<and>
-                                      insert_nth y B (insert_nth n S \<Gamma>1) \<turnstile> \<lparr>shift_L 1 (Suc n) t2|;|fill \<sigma>\<rparr> |:| C"
-       using  has_type_Case(4)[OF has_type_Case(7),of "Suc n", unfolded length_insert_nth]
-             has_type_Case(6)[OF has_type_Case(7),of "Suc n", unfolded length_insert_nth]  
-             has_type_Case(8) insert_nth_comp(2)[of n \<Gamma>1 _ S _] 
+    have B4: "\<not> n \<le> x \<Longrightarrow> \<not> n \<le> y \<Longrightarrow> insert_nth x A (insert_nth n S \<Gamma>1) \<turnstile> \<lparr>shift_L 1 (Suc n) t1|;|\<sigma>1\<rparr> |:| C \<and>
+                                      insert_nth y B (insert_nth n S \<Gamma>1) \<turnstile> \<lparr>shift_L 1 (Suc n) t2|;|\<sigma>1\<rparr> |:| C"
+       using has_type_Case(5)[of "Suc n", unfolded length_insert_nth]
+             has_type_Case(6)[of "Suc n", unfolded length_insert_nth]  
+             has_type_Case(7) insert_nth_comp(2)[of n \<Gamma>1 _ S _] 
       by (metis Suc_le_mono not_le)+
 
     show ?case
-      (*by (auto)(insert Sum_type B1 B2 B3 B4 "has_type_L.intros"(27), force+)*) sorry
+      using has_type_Case(4)[OF has_type_Case(7)]
+            has_type_L.intros(22) B1 B2 B3 B4
+      by force      
 next
   case (has_type_CaseV L I TL LT \<Gamma> t \<sigma>1 A)
     have branches_wtyped:"\<forall>i<length L.
        insert_nth (map (\<lambda>x. if n \<le> x then nat (int x + 1) else x) I ! i) (TL ! i) (take n \<Gamma> @ drop n \<Gamma> |,| S)
-       \<turnstile> \<lparr>((indexed_map 0 (\<lambda>k. shift_L 1 (if (I!k)<n then Suc n else n)) LT) ! i)|;|fill \<sigma>\<rparr> |:| A"
+       \<turnstile> \<lparr>((indexed_map 0 (\<lambda>k. shift_L 1 (if (I!k)<n then Suc n else n)) LT) ! i)|;| \<sigma>1\<rparr> |:| A"
       proof (rule+)
         fix i
         assume H:"i<length L"
         have P:"\<And>k. k\<le>length (insert_nth (I ! i) (TL ! i) \<Gamma>) \<Longrightarrow>
-                     insert_nth k S (insert_nth (I ! i) (TL ! i) \<Gamma>) \<turnstile> \<lparr>shift_L 1 k (LT ! i)|;|fill \<sigma>\<rparr>|:| A"
-          using has_type_CaseV(7,8) H 
+                     insert_nth k S (insert_nth (I ! i) (TL ! i) \<Gamma>) \<turnstile> \<lparr>shift_L 1 k (LT ! i)|;|\<sigma>1\<rparr>|:| A"
+          using has_type_CaseV(7) H 
           by auto
 
-        then have branches_type_n:"insert_nth n S (insert_nth (I ! i) (TL ! i) \<Gamma>) \<turnstile> \<lparr>shift_L 1 n (LT ! i)|;|fill \<sigma>\<rparr> |:| A"
-          using  has_type_CaseV(9)    
+        then have branches_type_n:"insert_nth n S (insert_nth (I ! i) (TL ! i) \<Gamma>) \<turnstile> \<lparr>shift_L 1 n (LT ! i)|;| \<sigma>1\<rparr> |:| A"
+          using  has_type_CaseV(8)    
                  length_insert_nth[of "I!i" "TL!i" \<Gamma>]
           by (metis le_SucI)
 
-        have branches_type_Sucn:"insert_nth (Suc n) S (insert_nth (I ! i) (TL ! i) \<Gamma>) \<turnstile> \<lparr>shift_L 1 (Suc n) (LT ! i)|;|fill \<sigma>\<rparr> |:| A"
-          using  has_type_CaseV(9)
+        have branches_type_Sucn:"insert_nth (Suc n) S (insert_nth (I ! i) (TL ! i) \<Gamma>) \<turnstile> \<lparr>shift_L 1 (Suc n) (LT ! i)|;|\<sigma>1\<rparr> |:| A"
+          using  has_type_CaseV(8)
                  length_insert_nth[of "I!i" "TL!i" \<Gamma>] P[of "Suc n"]
           by (metis Suc_le_mono)
 
         have 1:"n\<le> I!i \<Longrightarrow> insert_nth (map (\<lambda>x. if n \<le> x then nat (int x + 1) else x) I ! i) (TL ! i) (take n \<Gamma> @ drop n \<Gamma> |,| S)
-                \<turnstile> \<lparr>((indexed_map 0 (\<lambda>k. shift_L 1 (if (I!k)<n then Suc n else n)) LT) ! i)|;|fill \<sigma>\<rparr> |:| A"
-          using has_type_CaseV(1,2,9) H        
+                \<turnstile> \<lparr>((indexed_map 0 (\<lambda>k. shift_L 1 (if (I!k)<n then Suc n else n)) LT) ! i)|;|\<sigma>1\<rparr> |:| A"
+          using has_type_CaseV(1,2,8) H        
           proof -
             
             assume hyps:"n \<le> I ! i" "L \<noteq> \<emptyset>" "length I = length L" "n \<le> length \<Gamma>" "i < length L"
@@ -590,7 +466,7 @@ next
               by (simp add: index_not_index_cong[of 0 "\<lambda>k. shift_L 1 (if I ! k < n then Suc n else n)" LT, simplified])
             
             from branches_type_n
-              have "insert_nth (Suc (I ! i)) (TL ! i) (take n \<Gamma> @ drop n \<Gamma> |,| S) \<turnstile> \<lparr>shift_L 1 n (LT ! i)|;|fill \<sigma>\<rparr> |:| A"
+              have "insert_nth (Suc (I ! i)) (TL ! i) (take n \<Gamma> @ drop n \<Gamma> |,| S) \<turnstile> \<lparr>shift_L 1 n (LT ! i)|;|\<sigma>1\<rparr> |:| A"
                 using insert_nth_comp(1)[OF hyps(4,1)] H has_type_CaseV(4)
                 by force
             
@@ -599,8 +475,8 @@ next
           qed
 
         have  "\<not> n\<le> I!i \<Longrightarrow> insert_nth (map (\<lambda>x. if n \<le> x then nat (int x + 1) else x) I ! i) (TL ! i) (take n \<Gamma> @ drop n \<Gamma> |,| S)
-                \<turnstile> \<lparr>((indexed_map 0 (\<lambda>k. shift_L 1 (if (I!k)<n then Suc n else n)) LT) ! i)|;|fill \<sigma>\<rparr> |:| A"
-          using has_type_CaseV(1,2,9) H        
+                \<turnstile> \<lparr>((indexed_map 0 (\<lambda>k. shift_L 1 (if (I!k)<n then Suc n else n)) LT) ! i)|;|\<sigma>1\<rparr> |:| A"
+          using has_type_CaseV(1,2,8) H        
           proof -            
             assume hyps:"\<not>n \<le> I ! i" "L \<noteq> \<emptyset>" "length I = length L" "n \<le> length \<Gamma>" "i < length L"
             
@@ -610,7 +486,7 @@ next
               by (simp add: index_not_index_cong[of 0 "\<lambda>k. shift_L 1 (if I ! k < n then Suc n else n)" LT, simplified])
             
             from branches_type_Sucn
-              have  "insert_nth (I ! i) (TL ! i) (take n \<Gamma> @ drop n \<Gamma> |,| S) \<turnstile> \<lparr>shift_L 1 (Suc n) (LT ! i)|;|fill \<sigma>\<rparr> |:| A"
+              have  "insert_nth (I ! i) (TL ! i) (take n \<Gamma> @ drop n \<Gamma> |,| S) \<turnstile> \<lparr>shift_L 1 (Suc n) (LT ! i)|;|\<sigma>1\<rparr> |:| A"
                 using insert_nth_comp(2)[OF hyps(4), of "I!i"] hyps(1)[unfolded not_le[of n "I!i"]]
                 by fastforce
 
@@ -619,17 +495,14 @@ next
           qed
 
         with 1 show "insert_nth (map (\<lambda>x. if n \<le> x then nat (int x + 1) else x) I ! i) (TL ! i) (take n \<Gamma> @ drop n \<Gamma> |,| S)
-         \<turnstile> \<lparr>((indexed_map 0 (\<lambda>k. shift_L 1 (if (I!k)<n then Suc n else n)) LT) ! i)|;|fill \<sigma>\<rparr> |:| A"
+         \<turnstile> \<lparr>((indexed_map 0 (\<lambda>k. shift_L 1 (if (I!k)<n then Suc n else n)) LT) ! i)|;| \<sigma>1\<rparr> |:| A"
           by blast
       qed 
     show ?case
       using has_type_CaseV(1-4) index_not_index_cong[of 0 "\<lambda>k. shift_L 1 (if I ! k < n then Suc n else n)" LT]
-            has_type_CaseV(6)[OF has_type_CaseV(8,9)]
-            branches_wtyped
-      (*by (force intro!: has_type_L.intros(29))+     *) sorry
-next
-  case (has_type_PatternVar)
-    thus ?case sorry
+            has_type_CaseV(6)[OF has_type_CaseV(8)]
+            branches_wtyped            
+      by (force intro!: has_type_L.intros(24))
 qed (auto intro!: has_type_L.intros simp: nth_append min_def)
 
 lemma fill_keep_value:
@@ -641,10 +514,11 @@ lemma canonical_forms:
   "is_value_L v \<Longrightarrow> \<Gamma> \<turnstile> \<lparr>v|;|\<sigma>\<rparr> |:| T1 \<rightarrow> T2 \<Longrightarrow> \<exists>t n. v = LAbs T1 t"
   "is_value_L v \<Longrightarrow> \<Gamma> \<turnstile> \<lparr>v|;|\<sigma>\<rparr> |:| Unit \<Longrightarrow> v = unit"
   "is_value_L v \<Longrightarrow> \<Gamma> \<turnstile> \<lparr>v|;|\<sigma>\<rparr> |:| A |\<times>| B \<Longrightarrow> \<exists>v1 v2. is_value_L v1 \<and> is_value_L v2 \<and> v= \<lbrace>v1,v2\<rbrace>"
-  "is_value_L v \<Longrightarrow> \<Gamma> \<turnstile> \<lparr>v|;|\<sigma>\<rparr> |:| \<lparr>TL\<rparr> \<Longrightarrow> \<exists>L. is_value_L (Tuple L) \<and> v = Tuple L"
-  "is_value_L v \<Longrightarrow> \<Gamma> \<turnstile> \<lparr>v|;|\<sigma>\<rparr> |:| \<lparr>L|:|TL\<rparr> \<Longrightarrow> \<exists>L LT. is_value_L (Record L LT) \<and> v = (Record L LT)" 
-  "is_value_L v \<Longrightarrow> \<Gamma> \<turnstile> \<lparr>v|;|\<sigma>\<rparr> |:| A|+|B \<Longrightarrow> (\<exists>v1. is_value_L v1 \<and> v = inl v1 as A|+|B) \<or> (\<exists>v1. v = inr v1 as A|+|B \<and> is_value_L v1)" 
-  "is_value_L v \<Longrightarrow> \<Gamma> \<turnstile> \<lparr>v|;|\<sigma>\<rparr> |:| Nat \<Longrightarrow> \<exists>n. v = LNat n"
+  "is_value_L v \<Longrightarrow> \<Gamma> \<turnstile> \<lparr>v|;|\<sigma>\<rparr> |:| \<lparr>TL\<rparr> \<Longrightarrow> \<exists>L. is_value_L (Tuple L) \<and> v = Tuple L \<and> length TL = length L"
+  "is_value_L v \<Longrightarrow> \<Gamma> \<turnstile> \<lparr>v|;|\<sigma>\<rparr> |:| \<lparr>L|:|TL\<rparr> \<Longrightarrow> \<exists>LT. is_value_L (Record L LT) \<and> v = (Record L LT)" 
+  "is_value_L v \<Longrightarrow> \<Gamma> \<turnstile> \<lparr>v|;|\<sigma>\<rparr> |:| A|+|B \<Longrightarrow> (\<exists>v1. is_value_L v1 \<and> v = inl v1 as A|+|B) \<or> (\<exists>v1. v = inr v1 as A|+|B \<and> is_value_L v1)"
+  "is_value_L v \<Longrightarrow> \<Gamma> \<turnstile> \<lparr>v|;|\<sigma>\<rparr> |:| \<lambda>List A \<Longrightarrow> (v = Lnil A) \<or> (\<exists>v1 v2. is_value_L v1 \<and> is_value_L v2 \<and>
+                                                                v = Lcons A v1 v2)"
 proof -
   assume  val: "is_value_L v" and 
           typed: "\<Gamma> \<turnstile> \<lparr>v|;|\<sigma>\<rparr> |:| A|+|B"
@@ -652,5 +526,55 @@ proof -
     using val typed
     by (induction rule: is_value_L.induct, auto elim: "has_type_L.cases")
 qed (auto elim: "is_value_L.cases" "has_type_L.cases")  
+
+lemma progress:
+  "\<emptyset> \<turnstile> \<lparr>t|;|empty\<rparr> |:| A \<Longrightarrow> is_value_L t \<or> (\<exists>t1. eval1_L t t1)"
+proof (induction "\<emptyset>::ltype list" t "empty::nat\<rightharpoonup>ltype" A rule: has_type_L.induct)
+  case (has_type_LIf t1 t2 A t3)
+    thus ?case by (metis eval1_L.intros canonical_forms)
+next
+  case (has_type_LetPattern)
+    thus ?case sorry
+next
+  case (has_type_Tuple L TL)
+    note hyps=this
+    have "(\<exists>j<length L. (\<forall>i<j. is_value_L (L ! i)) \<and> (\<exists>t1. eval1_L (L ! j) t1))\<or>
+          is_value_L (Tuple L)"
+      
+      sorry
+    thus ?case sorry
+next
+  case (has_type_RCD)
+    thus ?case sorry
+next
+  case (has_type_ProjT i TL t)
+   thus ?case 
+     by (metis eval1_L.intros canonical_forms)     
+next
+  case (has_type_CaseV L I TL LT t A)
+    note hyps=this
+    show ?case
+      sorry
+next
+  case (has_type_head t A)
+    note hyps=this
+    show ?case
+      using canonical_forms(8)[OF _ hyps(1)]
+            hyps(2)
+      sorry
+next
+  case (has_type_tail t A)
+     note hyps=this
+    show ?case
+      using canonical_forms(8)[OF _ hyps(1)]
+            hyps(2)
+      sorry
+next
+  case (has_type_Variant t TL i)
+    thus ?case sorry
+next
+  case (has_type_isNil)
+    thus ?case sorry
+qed (force intro!: is_value_L.intros eval1_L.intros dest: canonical_forms)+
 
 end
